Refactor control pi-calculus to use the graph library and de Bruijn levels

theories/Pi/Control.v
@@ -10,58 +10,70 @@ Require Import Equality.
 Require Import Local.Prelude.
 Require Import Local.AbstractRewriting.
 Require Import Local.Substitution.
+Require Import Local.Pi.Graph.
 Require Import Local.Pi.Calculus.
 
 Set Primitive Projections.
 
-Local Notation nodes := (list (option type)).
+(* Typing judgements in the linear pi-calculus, and in subsets such as the
+   control pi-calculus, need an additional graph structure on names to enforce
+   acyclicity. We'll represent this by using an algebraic graph with pairs of
+   de Bruijn *level* and type as vertices. *)
 
-Definition has_input_type (g: nodes) (n: nat): Prop :=
+Definition env: Set :=
+  graph (nat * type).
+
+Definition env_type (g: env) (n: nat) (t: type) :=
+  has_vertex g (n, t).
+
+Definition has_input_type (g: env) (n: nat): Prop :=
   exists ts,
-  nth n g None = Some (channel I ts).
+  env_type g n (channel I ts).
 
-Definition has_output_type (g: nodes) (n: nat): Prop :=
+Definition has_output_type (g: env) (n: nat): Prop :=
   exists ts,
-  nth n g None = Some (channel O ts).
+  env_type g n (channel O ts).
 
-Record env: Type := env_mk {
-  env_nodes:
-    nodes;
-  env_edges:
-    relation nat
-}.
+Definition has_free_name (g: env) (n: nat): Prop :=
+  exists t,
+  env_type g n t.
 
-Global Coercion env_nodes: env >-> list.
+Definition env_edge (g: env) (i: nat) (j: nat): Prop :=
+  exists t u,
+  has_edge g (i, t) (j, u).
 
 Record env_wellformed (g: env): Prop := {
   env_wellformed_domain:
     forall i j,
-    env_edges g i j ->
+    env_edge g i j ->
     has_input_type g i;
   env_wellformed_codomain:
     forall i j,
-    env_edges g i j ->
+    env_edge g i j ->
     has_output_type g j;
+  env_wellformed_unique:
+    forall t u i,
+    env_type g i t ->
+    env_type g i u ->
+    t = u;
   env_wellformed_acyclic:
-    well_founded (env_edges g)
+    well_founded (env_edge g)
 }.
 
-Definition env_empty: env := {|
-  env_nodes := [];
-  env_edges x y := False
-|}.
-
-Lemma env_empty_is_wellformed:
-  env_wellformed env_empty.
+Lemma empty_is_wellformed:
+  env_wellformed empty.
 Proof.
   constructor; intros.
   - exfalso.
+    destruct H as (t, (u, ?)).
+    inversion H.
+  - exfalso.
+    destruct H as (t, (u, ?)).
     inversion H.
   - exfalso.
     inversion H.
-  - constructor.
-    intros b ?.
-    exfalso.
+  - constructor; intros.
+    destruct H as (t, (u, ?)).
     inversion H.
 Qed.
 
@@ -99,18 +111,9 @@ Lemma type_composition_is_a_function:
 Proof.
   intros.
   dependent destruction H.
-  - dependent destruction H2.
-    + now subst.
-    + now subst.
-    + now subst.
-  - dependent destruction H2.
-    + now subst.
-    + now subst.
-    + now subst.
-  - dependent destruction H2.
-    + now subst.
-    + now subst.
-    + now subst.
+  - dependent destruction H2; now subst.
+  - dependent destruction H2; now subst.
+  - dependent destruction H2; now subst.
 Qed.
 
 Lemma type_composition_is_commutative:
@@ -124,542 +127,225 @@ Proof.
   - now apply type_composition_oo with ts.
 Qed.
 
-Definition type_coherent: relation type :=
-  fun t1 t2 =>
-    exists t3, type_composition t1 t2 t3.
-
-Goal
-  ~(type_coherent (channel I []) (channel I [])).
-Proof.
-  intro.
-  destruct H.
-  dependent destruction H.
-Qed.
-
-Lemma type_coherent_sym:
-  symmetric type_coherent.
-Proof.
-  intros t1 t2 ?.
-  destruct H as (t3, ?).
-  exists t3.
-  now apply type_composition_is_commutative.
-Qed.
-
-Record env_coherent (g: env) (h: env): Prop := {
+Record env_coherent (g1: env) (g2: env): Prop := {
   env_coherent_pointwise:
     forall i t1 t2,
-    nth i g None = Some t1 ->
-    nth i h None = Some t2 ->
-    type_coherent t1 t2;
+    env_type g1 i t1 ->
+    env_type g2 i t2 ->
+    exists t3,
+    type_composition t1 t2 t3;
   env_coherent_acyclic:
-    well_founded (union (env_edges g) (env_edges h))
+    well_founded (union (env_edge g1) (env_edge g2))
 }.
 
-Inductive env_composition_nodes: nodes -> nodes -> nodes -> Prop :=
-  | env_composition_nodes_nil_left:
-    forall h,
-    env_composition_nodes [] h h
-  | env_composition_nodes_nil_right:
-    forall g,
-    env_composition_nodes g [] g
-  | env_composition_nodes_cons_left:
-    forall g h i t,
-    env_composition_nodes g h i ->
-    env_composition_nodes (t :: g) (None :: h) (t :: i)
-  | env_composition_nodes_cons_right:
-    forall g h i t,
-    env_composition_nodes g h i ->
-    env_composition_nodes (None :: g) (t :: h) (t :: i)
-  | env_composition_nodes_cons_compose:
-    forall g h i t1 t2 t3,
-    env_composition_nodes g h i ->
-    type_composition t1 t2 t3 ->
-    env_composition_nodes (Some t1 :: g) (Some t2 :: h) (Some t3 :: i).
+Axiom env_composition: env -> env -> env.
 
-Lemma env_composition_nodes_is_a_function:
-  forall g h i1,
-  env_composition_nodes g h i1 ->
-  forall i2,
-  env_composition_nodes g h i2 ->
-  i1 = i2.
+Inductive env_composition_vertex: env -> env -> nat -> type -> Prop :=
+  | env_composition_left:
+    forall g1 g2 n t,
+    env_type g1 n t ->
+    ~has_free_name g2 n ->
+    env_composition_vertex g1 g2 n t
+  | env_composition_right:
+    forall g1 g2 n t,
+    env_type g2 n t ->
+    ~has_free_name g1 n ->
+    env_composition_vertex g1 g2 n t
+  | env_composition_both:
+    forall g1 g2 n t u v,
+    env_type g1 n t ->
+    env_type g2 n u ->
+    type_composition t u v ->
+    env_composition_vertex g1 g2 n v.
+
+Lemma env_composition_vertex_inversion:
+  forall g1 g2 n t,
+  env_type (env_composition g1 g2) n t <-> env_composition_vertex g1 g2 n t.
 Proof.
-  induction 1; intros.
-  - now dependent destruction H.
-  - now dependent destruction H.
-  - dependent destruction H0.
-    + f_equal.
-      now apply IHenv_composition_nodes.
-    + f_equal.
-      now apply IHenv_composition_nodes.
-  - dependent destruction H0.
-    + f_equal.
-      now apply IHenv_composition_nodes.
-    + f_equal.
-      now apply IHenv_composition_nodes.
-  - dependent destruction H1.
-    assert (t3 = t5) by now apply type_composition_is_a_function with t1 t2.
-    subst; f_equal.
-    now apply IHenv_composition_nodes.
-Qed.
+  split; intros.
+  - admit.
+  - admit.
+Admitted.
 
-Lemma env_composition_nodes_is_commutative:
-  forall g h i,
-  env_composition_nodes g h i ->
-  env_composition_nodes h g i.
+Lemma env_composition_preserves_wellformedness:
+  forall g1 g2,
+  env_coherent g1 g2 ->
+  env_wellformed g1 ->
+  env_wellformed g2 ->
+  env_wellformed (env_composition g1 g2).
 Proof.
-  induction 1.
-  - constructor.
-  - constructor.
-  - now constructor.
-  - now constructor.
-  - constructor.
-    + assumption.
-    + now apply type_composition_is_commutative.
-Qed.
-
-Lemma env_composition_nodes_input_inversion:
-  forall g h i,
-  env_composition_nodes g h i ->
-  forall x ts,
-  nth x g None = Some (channel I ts) ->
-  nth x i None = Some (channel I ts).
-Proof.
-  induction 1; intros.
-  - exfalso.
-    destruct x; inversion H.
-  - assumption.
-  - destruct x.
-    + assumption.
-    + simpl.
-      now apply IHenv_composition_nodes.
-  - destruct x.
-    + exfalso.
-      inversion H0.
-    + simpl.
-      now apply IHenv_composition_nodes.
-  - destruct x.
-    + simpl in H1 |- *.
-      (* We have a composition of t1 and t2 into t3; since t1 is an input type,
-         it means that t3 also has to be an input type, and t2 had to be a dual
-         output type. *)
-      dependent destruction H1.
-      dependent destruction H0.
-      reflexivity.
-    + simpl.
-      now apply IHenv_composition_nodes.
-Qed.
-
-Inductive env_composition_edges: env -> env -> nodes -> relation nat :=
-  | env_composition_edges_mk:
-    forall g h i x y,
-    let R := union (env_edges g) (env_edges h) in
-    t(R) x y ->
-    env_composition_nodes g h i ->
-    has_input_type i x ->
-    has_output_type i y ->
-    env_composition_edges g h i x y.
-
-Inductive env_composition: env -> env -> env -> Prop :=
-  | env_composition_mk:
-    forall g h i R,
-    same_relation R (env_composition_edges g h i) ->
-    env_composition_nodes g h i ->
-    env_composition g h (env_mk i R).
-
-Goal
-  forall g h,
-  env_coherent g h ->
-  exists i,
-  env_composition g h i.
-Proof.
-  destruct 1 as (?H, ?H).
-  assert (exists i, env_composition_nodes g h i) as (i, ?).
-  - clear H0.
-    destruct g as (g, R).
-    destruct h as (h, S).
-    simpl in H |- *; clear R S.
-    generalize dependent h.
-    induction g; intros.
-    + eexists; constructor.
-    + destruct h.
-      * eexists; constructor.
-      * destruct IHg with h as (i, ?); intros.
-        --- apply H with (S i); now simpl.
-        --- destruct a, o.
-            +++ destruct H with 0 t t0 as (?t, ?); simpl; auto.
-                eexists; constructor.
-                *** eassumption.
-                *** eassumption.
-            +++ eexists; constructor.
-                eassumption.
-            +++ eexists; constructor.
-                eassumption.
-            +++ eexists; constructor.
-                eassumption.
-  - set (R := env_composition_edges g h i).
-    assert (same_relation R R) by firstorder.
-    exists (env_mk i R).
-    now constructor.
-Qed.
-
-Lemma env_composition_edges_switch:
-  forall g h i,
-  inclusion (env_composition_edges g h i) (env_composition_edges h g i).
-Proof.
-  intros g h i x y ?.
-  destruct H.
-  econstructor.
-  - clear H0 H1 H2.
-    induction H.
-    + apply t_step.
-      destruct H; firstorder.
-    + now apply t_trans with y.
-  - now apply env_composition_nodes_is_commutative.
-  - eassumption.
-  - eassumption.
-Qed.
-
-Lemma env_composition_edges_is_commutative:
-  forall g h i,
-  inclusion (env_composition_edges g h i) (env_composition_edges h g i).
-Proof.
-  intros g h i x y ?.
-  destruct H; constructor.
-  - clear H0 H1 H2.
-    induction H.
-    + destruct H.
-      * auto with cps.
-      * auto with cps.
-    + eauto with cps.
-  - now apply env_composition_nodes_is_commutative.
-  - assumption.
-  - assumption.
-Qed.
-
-Lemma env_composition_is_commutative:
-  forall g h i,
-  env_composition g h i ->
-  env_composition h g i.
-Proof.
-  destruct 1.
-  constructor.
-  - split; intros x y ?.
-    + apply H in H1.
-      now apply env_composition_edges_is_commutative.
-    + apply H.
-      now apply env_composition_edges_is_commutative.
-  - now apply env_composition_nodes_is_commutative.
-Qed.
-
-Lemma env_conherence_implies_wellformedness:
-  forall g h,
-  env_coherent g h ->
-  forall i,
-  env_composition g h i ->
-  env_wellformed i.
-Proof.
-  intros.
-  destruct H as (?H, ?H).
-  constructor.
-  - intros x y ?.
-    destruct H0.
-    apply H0 in H2.
-    destruct H2.
-    assumption.
-  - intros x y ?.
-    destruct H0.
-    apply H0 in H2.
-    destruct H2.
-    assumption.
-  - destruct H0.
-    intros x; simpl.
-    specialize (H1 x).
-    set (S := union (env_edges g) (env_edges h)) in H1.
-    replace (Acc S) with (SN (transp S)) in H1 by auto.
-    induction H1 using SN_ind.
-    constructor; intros y ?.
-    apply H3; clear H2.
-    apply H0 in H4; clear H0.
-    destruct H4.
-    clear H1 H2 H3 H4 H5.
-    induction H0.
-    + destruct H0.
-      * apply t_step.
-        now left.
-      * apply t_step.
-        now right.
-    + eauto with cps.
-Qed.
+  constructor; intros.
+  - destruct H2 as (t, (u, ?)).
+    admit.
+  - destruct H2 as (t, (u, ?)).
+    admit.
+  - (* We check the inversion hypothesis for the existence of the vertices
+       [i: t] and [i: u] in the composition. This is mostly straightforward, as
+       it will either exist in [g1] and not [g2], or the other way around. In
+       the case that it exists in both, uniqueness follows from the fact that
+       type composition itself is unique. *)
+    apply env_composition_vertex_inversion in H2.
+    apply env_composition_vertex_inversion in H3.
+    destruct H2, H3.
+    + firstorder.
+    + firstorder.
+    + firstorder.
+    + firstorder.
+    + firstorder.
+    + firstorder.
+    + firstorder.
+    + firstorder.
+    + assert (t0 = t) by now apply env_wellformed_unique with g1 n.
+      assert (u0 = u) by now apply env_wellformed_unique with g2 n.
+      subst; now apply type_composition_is_a_function with t u.
+  - (* It's not true that composition preserves acyclicity of the graphs. The
+       proof comes directly from the hypothesis that they are coherent. We play
+       a simple bisimulation game. *)
+    intro x; apply env_coherent_acyclic in H.
+    induction H with x.
+    constructor; intros.
+    admit.
+Admitted.
 
 (* -------------------------------------------------------------------------- *)
 
-Inductive env_hiding_edges: nat -> relation nat -> relation nat :=
-  | env_hiding_edges_mk:
-    forall (R: relation nat) n x y,
-    R (n + x) (n + y) ->
-    env_hiding_edges n R x y.
+(* Whenever we are removing something from an action type, we will remove some
+   number of the most recently introduced variables simultaneously. In order to
+   implement that, since we're using de Bruijn levels, we simply remove all the
+   vertices that have a level higher then some number. *)
 
-Inductive env_hiding: nat -> env -> env -> Prop :=
-  | env_hiding_mk:
-    forall n g R S h,
-    drop 0 n g h ->
-    same_relation S (env_hiding_edges n R) ->
-    env_hiding n (env_mk g R) (env_mk h S).
+Definition env_hiding (g: env) (n: nat): env :=
+  (* Keep vertices smaller or equal to n. *)
+  graph_induce (fun v => n <=? fst v) g.
 
 Lemma env_hiding_preserves_wellformedness:
-  forall n g h,
-  env_wellformed g ->
-  env_hiding n g h ->
-  env_wellformed h.
-Proof.
-  constructor; intros.
-  - destruct H as (?H, _, _).
-    destruct H0; simpl in *.
-    apply H2 in H1.
-    destruct H1.
-    specialize (H _ _ H1).
-    clear H1 H2 y.
-    dependent induction H0.
-    + assumption.
-    + now apply IHdrop.
-  - destruct H as (_, ?H, _).
-    destruct H0; simpl in *.
-    apply H2 in H1.
-    destruct H1.
-    specialize (H _ _ H1).
-    clear H1 H2 x.
-    dependent induction H0.
-    + assumption.
-    + now apply IHdrop.
-  - destruct H as (_, _, ?H).
-    destruct H0; simpl in *.
-    clear H0 h.
-    intros x.
-    specialize (H (n + x)).
-    replace (Acc R) with (SN (transp R)) in H by auto.
-    remember (n + x) as i.
-    generalize dependent x.
-    induction H using SN_ind.
-    intros; subst.
-    constructor; intros y ?.
-    eapply H2; eauto.
-    apply H1 in H0.
-    destruct H0.
-    apply t_step.
-    assumption.
-Qed.
-
-(* -------------------------------------------------------------------------- *)
-
-Definition env_singleton (n: nat) (t: type) := {|
-  env_nodes := repeat None n ++ [Some t];
-  env_edges x y := False
-|}.
-
-Definition env_singleton_holes:
-  forall i t n,
-  n <> i ->
-  nth i (env_singleton n t) None = None.
-Proof.
-  intros.
-  destruct (lt_eq_lt_dec n i) as [ [ ? | ? ] | ? ].
-  - unfold env_singleton; simpl.
-    rewrite app_nth2.
-    + rewrite repeat_length.
-      remember (i - n) as m.
-      destruct m.
-      * exfalso.
-        lia.
-      * now destruct m.
-    + rewrite repeat_length.
-      lia.
-  - exfalso.
-    contradiction.
-  - unfold env_singleton; simpl.
-    rewrite app_nth1.
-    + apply nth_repeat.
-    + now rewrite repeat_length.
-Qed.
-
-Definition env_singleton_is_always_coherent:
   forall g,
   env_wellformed g ->
-  forall n t,
-  nth n g None = None ->
-  env_coherent g (env_singleton n t).
+  forall n,
+  env_wellformed (env_hiding g n).
 Proof.
-  intros.
+  (* Removing edges doesn't break any of the desired properties. *)
   constructor; intros.
-  - exfalso.
-    destruct (Nat.eq_dec n i); subst.
-    + rewrite H0 in H1.
-      inversion H1.
-    + clear H0 H1 t1.
-      rewrite env_singleton_holes in H2.
-      * inversion H2.
+  - destruct H0 as (t, (u, ?)).
+    (* We removed some vertices from [g]. If, after that, we still have an edge
+       from [i: t] to [j: u], we can check that [i] was already present in [g],
+       and by our hypothesis, there are ts types such that [i: !ts] exists in
+       [g]. As, also by our hypothesis, associations are unique, [!ts] and [t]
+       are the same, and, since the resulting graph has a vertex [i: t] still,
+       we check that this vertex is indeed [i: !ts] as required. *)
+    destruct env_wellformed_domain with g i j as (ts, ?).
+    + assumption.
+    + exists t, u.
+      eapply graph_induce_reflects_edge.
+      eassumption.
+    + exists ts.
+      apply graph_vertex_from_edge_left with (j, u).
+      rewrite env_wellformed_unique with g (channel I ts) t i.
       * assumption.
-  - clear H0.
-    intros x.
-    apply env_wellformed_acyclic in H.
-    specialize (H x).
-    replace (Acc (env_edges g)) with (SN (transp (env_edges g))) in H by auto.
-    induction H using SN_ind.
-    constructor; intros y ?.
-    apply H2.
-    destruct H0.
-    + apply t_step.
-      assumption.
-    + exfalso.
-      inversion H0.
-Qed.
-
-Lemma env_singleton_composition_inversion:
-  forall n g t h,
-  env_composition_nodes g (env_singleton n t) h ->
-  forall k,
-  k <> n ->
-  nth k g None = nth k h None.
-Proof.
-  induction n; simpl; intros.
-  - dependent destruction H.
-    + destruct k; try lia.
-      now destruct k.
-    + destruct k; try lia.
-      now dependent destruction H.
-    + destruct k; try lia.
-      now dependent destruction H.
-  - destruct k.
-    + now dependent destruction H; simpl.
-    + assert (k <> n) by lia.
-      dependent destruction H; simpl.
-      * clear IHn H0.
-        generalize dependent k.
-        induction n; destruct k; simpl; intros.
-        --- exfalso; contradiction.
-        --- now destruct k.
-        --- reflexivity.
-        --- now erewrite <- IHn with k by lia.
-      * now apply IHn with t.
-      * now apply IHn with t.
+      * assumption.
+      * assumption.
+      * apply graph_vertex_from_edge_left with (j, u).
+        eapply graph_induce_reflects_edge.
+        eassumption.
+  - (* Same reasoning as above, accordingly. *)
+    destruct H0 as (t, (u, ?)).
+    destruct env_wellformed_codomain with g i j as (ts, ?).
+    + assumption.
+    + exists t, u.
+      eapply graph_induce_reflects_edge.
+      eassumption.
+    + exists ts.
+      apply graph_vertex_from_edge_right with (i, t).
+      rewrite env_wellformed_unique with g (channel O ts) u j.
+      * assumption.
+      * assumption.
+      * assumption.
+      * apply graph_vertex_from_edge_right with (i, t).
+        eapply graph_induce_reflects_edge.
+        eassumption.
+  - (* Hiding can't add any new vertex. If both [i: t] and [i: u] already
+       existed inside of [g], by our hypothesis they are the same thing. *)
+    apply env_wellformed_unique with g i.
+    + assumption.
+    + eapply graph_induce_reflects_vertex.
+      eassumption.
+    + eapply graph_induce_reflects_vertex.
+      eassumption.
+  - (* Since [g] is acyclic, we can't possibly get a cycle by just removing
+       some vertices. We start from an arbitrary vertex [x]. If the opponent can
+       give us an [y] such that a vertex exists in the resulting graph from [x]
+       to [y], we can check that it already existed in [g] and keep following
+       the same path, known to be terminating. We win the game once the opponent
+       can't find more edges, either because it reached the same end as in [g]
+       or possibly earlier if it reached a removed vertex. *)
+    intro x.
+    induction env_wellformed_acyclic with g x; auto.
+    constructor; intros y (t, (u, ?)).
+    apply H1; exists t, u.
+    eapply graph_induce_reflects_edge.
+    eassumption.
 Qed.
 
 (* -------------------------------------------------------------------------- *)
+
+Definition env_singleton (n: nat) (t: type): env :=
+  vertex (n, t).
+
+Lemma env_singleton_is_wellformed:
+  forall n t,
+  env_wellformed (env_singleton n t).
+Proof.
+  constructor; intros.
+  - (* There are no edges. *)
+    exfalso.
+    destruct H as (u, (v, ?)).
+    inversion H.
+  - (* Still no edges. *)
+    exfalso.
+    destruct H as (u, (v, ?)).
+    inversion H.
+  - (* There's a single vertex, clearly it's equal to itself. *)
+    unfold env_singleton, env_type in H, H0.
+    dependent destruction H.
+    dependent destruction H0.
+    reflexivity.
+  - (* Hey! Still no edges! Instant win in the bisimulation game. *)
+    intro x.
+    constructor; intros y (u, (v, ?)).
+    exfalso.
+    inversion H.
+Qed.
+
+(* -------------------------------------------------------------------------- *)
+
+(* A variable is said to be active if it is associated to some type in the graph
+   and it has no edge pointing to it. *)
 
 Definition active (g: env) (y: nat): Prop :=
   exists2 t,
-  nth y g None = Some t & (forall x, ~env_edges g x y).
+  env_type g y t & (forall x, ~env_edge g x y).
 
-Goal
+(* TODO: do we need this one? *)
+
+Lemma input_type_is_always_active:
   forall g y,
   env_wellformed g ->
   has_input_type g y ->
   active g y.
 Proof.
-  intros g y ?H (ts1, ?).
-  exists (channel I ts1).
+  intros.
+  destruct H0 as (ts1, ?).
+  exists (channel I ts1); intros.
   - assumption.
-  - intros x ?H.
+  - intro.
     apply env_wellformed_codomain in H1 as (ts2, ?).
-    + rewrite H0 in H1.
-      inversion H1.
+    + assert (channel I ts1 = channel O ts2).
+      * now apply env_wellformed_unique with g y.
+      * inversion H2.
     + assumption.
 Qed.
 
-Inductive env_prefix_edges: nat -> nodes -> relation nat :=
-  | env_prefix_edges_mk:
-    forall n g y,
-    active g y ->
-    has_output_type g y ->
-    env_prefix_edges n g n y.
-
-Inductive env_prefix: nat -> type -> env -> env -> Prop :=
-  | env_prefix_mk:
-    forall n t g h R S,
-    alternating I t ->
-    nth n (env_nodes g) None = None ->
-    env_composition g (env_singleton n t) h ->
-    same_relation S (union R (env_prefix_edges n g)) ->
-    env_prefix n t (env_mk g R) (env_mk h S).
-
-Lemma env_prefix_preserves_wellformedness:
-  forall n t g h,
-  env_prefix n t g h ->
-  env_wellformed g ->
-  env_wellformed h.
-Proof.
-  intros.
-  destruct H.
-  constructor; intros.
-  - destruct H0 as (?H, _, _); simpl in *.
-    apply H3 in H4 as [ ?H | ?H ].
-    + rename i into x, j into y.
-      apply H0 in H4 as (ts, ?).
-      destruct H2; simpl.
-      exists ts.
-      now apply env_composition_nodes_input_inversion with g h.
-    + apply env_composition_is_commutative in H2.
-      assert (has_input_type (env_singleton n t) i) as (ts, ?).
-      * destruct H4.
-        dependent destruction H.
-        exists ts; simpl.
-        clear H1 H2 H3 H0 H4 H5 y.
-        induction n; eauto.
-      * destruct H2; simpl.
-        exists ts.
-        eapply env_composition_nodes_input_inversion; eauto.
-  - destruct H0 as (_, ?H, _); simpl in *.
-    assert (j <> n).
-    + intros ?H; subst.
-      apply H3 in H4 as [ ?H | ?H ].
-      * apply H0 in H4 as (ts, ?).
-        rewrite H1 in H4.
-        inversion H4.
-      * dependent destruction H4.
-        destruct H5 as (ts, ?).
-        rewrite x, H1 in H5.
-        inversion H5.
-    + apply H3 in H4 as [ ?H | ?H ].
-      * dependent destruction H2; simpl.
-        apply H4 in H5 as (ts, ?).
-        erewrite env_singleton_composition_inversion in H5; eauto.
-        now exists ts.
-      * dependent destruction H2; simpl.
-        dependent destruction H5; simpl.
-        destruct H6 as (ts, ?).
-        rewrite x in H6; clear x.
-        erewrite env_singleton_composition_inversion in H6; eauto.
-        now exists ts.
-  - destruct H0 as (?H, ?H, ?H); simpl in *.
-    intros x.
-    specialize (H5 x).
-    replace (Acc R) with (SN (transp R)) in H5 by auto.
-    induction H5 using SN_ind.
-    constructor; intros.
-    apply H3 in H7 as [ ? | ? ].
-    + apply H6.
-      apply t_step.
-      assumption.
-    + destruct H7 as (x, i, y, ?, ?).
-      clear H5 H6.
-      (* This has to be the last step. *)
-      constructor; intros z ?.
-      exfalso.
-      apply H3 in H5 as [ ? | ? ].
-      * apply H4 in H5 as (ts, ?).
-        rewrite H1 in H5.
-        inversion H5.
-      * destruct H5 as (_, j, z, ?, ?).
-        destruct H6 as (ts, ?).
-        rewrite H1 in H6.
-        inversion H6.
-Qed.
-
 (* -------------------------------------------------------------------------- *)
-
-Definition env_mode (m: mode) (g: nodes): Prop :=
-  forall i t,
-  nth i g None = Some t ->
-  get_mode t = m.
 
 Inductive mode_composition: mode -> mode -> mode -> Prop :=
   | mode_composition_io:
@@ -669,64 +355,81 @@ Inductive mode_composition: mode -> mode -> mode -> Prop :=
   | mode_composition_ii:
     mode_composition I I I.
 
+Definition env_mode (m: mode) (g: env): Prop :=
+  forall i t,
+  env_type g i t ->
+  get_mode t = m.
+
+(* -------------------------------------------------------------------------- *)
+
 Inductive typing: mode -> term -> env -> Prop :=
-  (*
-    -------------- (ZERO)
-      |-I 0 |>
-  *)
+  (* Rule for typing an inactive process:
+
+      ------------ (ZERO)
+        |-I 0 |>
+
+     The inactive process is only typeable in an empty action type, with input
+     mode (clearly, there's no active output). In order to add unused (output)
+     variables, we will use weakening. *)
   | typing_zero:
-    typing I inactive env_empty
+    typing I inactive empty
+  (* Rule for typing the composition of two processes:
 
-  (*
-      |-(m) p |> G    |-(n) q |> H    G >< H    G * H = I    m * n = o
-    -------------------------------------------------------------------- (PAR)
-                              |-(o) (p | q) |> I
+        |-(m) p |> G    |-(n) q |> H    G >< H
+      ------------------------------------------- (PAR)
+               |-(m * n) p | q |> G * H
 
-    TODO: maybe we should require that a composition only exists when the action
-    types are coherent with each other, as composition by itself does not imply
-    that there is no cycle in the resulting term.
-  *)
+     Parallel composition first assumes that [p] and [q] are typeable. We check
+     then that their action types, [G] and [H] respectively, are coherent with
+     each other in order to avoid cycles and multiple inputs on the same name.
+     We note that the modes must be able to be composed together, otherwise this
+     won't be defined (we don't add this explicitly in the hypotheses as Honda
+     et al. do). *)
   | typing_par:
-    forall m n o p q g h i,
+    forall m n o p q g h,
     typing m p g ->
     typing n q h ->
     env_coherent g h ->
-    env_composition g h i ->
     mode_composition m n o ->
-    typing o (parallel p q) i
+    typing o (parallel p q) (env_composition g h)
+  (* Rule for typing name restriction:
 
-  (*
-       |-(m) p |> G, x: !(ts)
-    ---------------------------- (RES)
-      |-(m) (x: !(ts))(p) |> G
-  *)
+         |-(m) p |> G     G(x) = ti
+      ------------------------------- (RES)
+           |-(m) (x: ti)p |> G/x
+
+     In order to type a restriction, we assume that [p] is typeable in some
+     action type [G] such that [x: ti] is a vertex within it. Note that this
+     will require that the name [x] is defined as a replicated input in [p]. *)
   | typing_res:
-    forall m p g h t,
+    forall m p g t,
     typing m p g ->
     alternating I t ->
-    nth 0 g None = Some t ->
-    env_hiding 1 g h ->
-    typing m (restriction t p) h
+    (* TODO: which level is variable 0...? *)
+    env_type g 42 t ->
+    typing m (restriction t p) (env_hiding g 42)
+  (* Rule for weakening, which is explicit:
 
-  (*
-           |-(m) p |> G
-    -------------------------- (WEAK)
-      |-(m) p |> G, x: ?(ts)
-  *)
+        |-(m) p |> G   x undefined in G
+      ----------------------------------- (WEAK)
+            |-(m) p |> G, x: ?(ts)
+
+     If [p] is typeable in some action type [G], it's also typeable in some
+     action type which extends [G] by adding a new vertex [x: t] if [x] isn't
+     defined in [G] and if [t] is an output type. Basically, it says that we may
+     ignore any unused free variables which have output types. *)
   | typing_weak:
-    forall m p g n t h,
+    forall m p g n t,
     typing m p g ->
     alternating O t ->
-    nth n g None = None ->
-    env_composition g (env_singleton n t) h ->
-    typing m p h
-
+    ~has_free_name g n ->
+    typing m p (env_composition g (env_singleton n t))
   (*
        |-O p |> G, ys: ts    md(G) = ?
     ------------------------------------- (IN)
       |-I !x(ys: ts).p |> x: !(ts) -> G
   *)
-  | typing_in:
+  (* | typing_in: (* TODO: fix this! *)
     forall p g n ts h i,
     typing O p g ->
     nth (length ts + n) g None = None ->
@@ -736,7 +439,35 @@ Inductive typing: mode -> term -> env -> Prop :=
        edge and thus all variables must be active. *)
     env_hiding (length ts) g h ->
     env_prefix n (channel I ts) h i ->
-    typing I (replication n ts p) i.
+    typing I (replication n ts p) i *)
+  (*
+    --------------------------------------- (FOUT)
+      |-O x<ys> |> (x: ?(ts)) * (ys: ~ts)
+
+    Note that in here we do not expect the names in ys to be all different, and,
+    because of that, if y_i = y_j, then we expect t_i = t_j.
+
+    It's also important to notice that we're not checking, individually, the
+    composition of each individual names. While this won't be a problem in here,
+    it would be in case we had linear types as in the linear pi-calculus studied
+    by Yoshida. If we are to consider the full thing, we might want to rework
+    this rule to cover this possibility.
+  *)
+  (* | typing_out:
+  *).
+
+(*
+Lemma typing_bout:
+  (*
+        |-I P |> A, ys: ts     A >< x: ?(ts)
+    -------------------------------------------- (BOUT)
+            |-O x[ys] p |> A * x: ?(ts)
+  *)
+*)
+
+Definition typed (p: term): Prop :=
+  exists m g,
+  typing m p g.
 
 Lemma typing_env_wellformed:
   forall m p g,
@@ -744,17 +475,11 @@ Lemma typing_env_wellformed:
   env_wellformed g.
 Proof.
   induction 1.
-  - apply env_empty_is_wellformed.
-  - now apply env_conherence_implies_wellformedness with g h.
-  - now apply env_hiding_preserves_wellformedness with 1 g.
-  - apply env_conherence_implies_wellformedness with g (env_singleton n t).
-    + apply env_singleton_is_always_coherent.
-      * assumption.
-      * assumption.
+  - apply empty_is_wellformed.
+  - now apply env_composition_preserves_wellformedness.
+  - now apply env_hiding_preserves_wellformedness.
+  - apply env_composition_preserves_wellformedness.
+    + admit.
     + assumption.
-  - apply env_prefix_preserves_wellformedness with n (channel I ts) h.
-    + assumption.
-    + apply env_hiding_preserves_wellformedness with (length ts) g.
-      * assumption.
-      * assumption.
-Qed.
+    + apply env_singleton_is_wellformed.
+Admitted.
